proofs/Gf2Algebra.lean
@@ -2,3 +2,4 @@ import Gf2Algebra.Types
 import Gf2Algebra.FunsExternal
 import Gf2Algebra.Funs
 import Gf2Algebra.Proofs.Bipedal3Correctness
+import Gf2Algebra.Proofs.Packed5Correctness
